src/lowparse/LowParse.Low.ConstInt32.fst
@@ -5,12 +5,15 @@ module LowParse.Low.ConstInt32
 include FStar.Endianness
 
 include LowParse.Spec.ConstInt32
+include LowParse.Low.Combinators
 
 include LowParse.Low.BoundedInt
 
 module U32 = FStar.UInt32
 module HS = FStar.HyperStack
 module HST = FStar.HyperStack.ST
+module B = LowStar.Buffer
+module Cast = FStar.Int.Cast
 
 let valid_constint32le
   (v: nat { 0 <= v /\ v < 4294967296 } )
@@ -26,26 +29,34 @@ let valid_constint32le
   valid_facts (parse_int32_le ()) h input pos;
   parse_constint32le_unfold v (bytes_of_slice_from h input pos)
 
-let read_int32_le : unit -> Tot (leaf_reader (parse_int32_le ()))
-= read_bounded_integer_le_4
+let read_int32_le : (leaf_reader (parse_int32_le ()))
+= make_total_constant_size_reader 4 4ul decode_int32_le (decode_int32_le_total_constant ()) (fun #rrel #rel b pos ->
+    let h = HST.get () in
+    [@inline_let] let _ = decode_int32_le_eq (Seq.slice (B.as_seq h b) (U32.v pos) (U32.v pos + 4)) in
+    let r0 = B.index b pos in
+    let r1 = B.index b (pos `U32.add` 1ul) in
+    let r2 = B.index b (pos `U32.add` 2ul) in
+    let r3 = B.index b (pos `U32.add` 3ul) in
+    Cast.uint8_to_uint32 r0 `U32.add` (256ul `U32.mul` (Cast.uint8_to_uint32 r1 `U32.add` (256ul `U32.mul` (Cast.uint8_to_uint32 r2 `U32.add` (256ul `U32.mul` Cast.uint8_to_uint32 r3)))))
+  )
 
-(*
+
 let validate_constint32le_slow
   (v: U32.t { 0 <= U32.v v /\ U32.v v < 4294967296 } )
 : Tot (validator (parse_constint32le (U32.v v)))
 = fun #rrel #rel (input: slice rrel rel) (pos: U32.t) ->
   let h = HST.get() in
     let _ =
-      valid_equiv (parse_constint32le (U32.v v)) h input pos;
-      valid_constint32le (U32.v v) h input pos    
+      valid_constint32le (U32.v v) h input pos;    
+      valid_equiv (parse_int32_le ()) h input pos
     in
   if U32.lt (input.len `U32.sub` pos) 4ul
   then
     validator_error_not_enough_data
   else
-    let v' = read_bounded_integer_le_4 input pos in
+    let v' = read_int32_le input pos in
     if U32.eq v v' then
       pos `U32.add` 4ul
     else
       validator_error_generic
-*)
+
